feat: Addressed some footnotes

src/main/translation/expression.scala
@@ -116,12 +116,7 @@ def translateBasicExpr(expr: Parsers.BasicExpr)(using context: Context): BasicEx
   // Therefore, that will need to be dealt with
   case Parsers.Cond(cond, Parsers.ExprBlock(Nil, thenBranch), Parsers.ExprBlock(Nil, Parsers.BoolLiteral(false))) => 
     Binary(BoolAnd, translateBasicExpr(cond), translateBasicExpr(thenBranch))
-  // case Parsers.Cond(cond, Parsers.ExprBlock(Nil, thenBranch), Parsers.ExprBlock(Nil, Parsers.BoolLiteral(true))) => 
-  //   Binary(BoolOr, Unary(Not, translateBasicExpr(cond)), translateBasicExpr(thenBranch))
-  // case Parsers.Cond(cond, Parsers.ExprBlock(Nil, Parsers.BoolLiteral(false)), Parsers.ExprBlock(Nil, elseBranch)) => 
-  //   Binary(BoolAnd, Unary(Not, translateBasicExpr(cond)), translateBasicExpr(elseBranch))
-  // case Parsers.Cond(cond, Parsers.ExprBlock(Nil, Parsers.BoolLiteral(true)), Parsers.ExprBlock(Nil, elseBranch)) => 
-  //   Binary(BoolOr, translateBasicExpr(cond), translateBasicExpr(elseBranch))
+
   case Parsers.Cond(Parsers.Not(cond), thenBranch, elseBranch) => 
     Cond(
       translateBasicExpr(cond),
